Stuck

src/specs/EvaluateLagrangePolyOutOfDomain.ec
@@ -1,12 +1,18 @@
 pragma Goals:printall.
 
-require        Constants.
+require import AllCore.
+require import Int.
+require import IntDiv.
+require import Constants.
+require import Utils.
 require import Modexp.
 require import PurePrimops.
 require import RevertWithMessage.
 require import UInt256.
 require import Verifier.
 require import YulPrimops.
+
+import MemoryMap.
 
 module EvaluateLagrangePolyOutOfDomain = {
   proc low(polyNum: uint256, at: uint256): uint256 = {
@@ -31,6 +37,48 @@ module EvaluateLagrangePolyOutOfDomain = {
     denominator <@ Modexp.low(denominator, ((W256.of_int Constants.R) - (W256.of_int 2)));
     ret <- (PurePrimops.mulmod ret denominator (W256.of_int Constants.R));
     return ret;
+  }
+
+  proc low'(polyNum: uint256, at: uint256): uint256 = {
+  var ret, omegaPower, tmp267, _10, denominator;
+    tmp267 <@ Modexp.low(at, (W256.of_int Constants.DOMAIN_SIZE));
+
+    omegaPower <- (W256.of_int 1);
+    if ((bool_of_uint256 polyNum))
+    {
+      omegaPower <@ Modexp.low((W256.of_int Constants.OMEGA), polyNum);
+    }
+    
+    ret <- (PurePrimops.addmod tmp267 ((W256.of_int Constants.R) - W256.one) (W256.of_int Constants.R));
+    if ((bool_of_uint256 (PurePrimops.iszero ret)))
+    {
+      RevertWithMessage.low(W256.of_int 28, W256.of_int STRING);
+    }
+    
+    ret <- (PurePrimops.mulmod ret omegaPower (W256.of_int Constants.R));
+    _10 <- ((W256.of_int Constants.R) - omegaPower);
+    denominator <- (PurePrimops.addmod at _10 (W256.of_int Constants.R));
+    denominator <- (PurePrimops.mulmod denominator (W256.of_int Constants.DOMAIN_SIZE) (W256.of_int Constants.R));
+    denominator <@ Modexp.low(denominator, ((W256.of_int Constants.R) - (W256.of_int 2)));
+    ret <- (PurePrimops.mulmod ret denominator (W256.of_int Constants.R));
+    return ret;
+  }
+  
+  proc mid(polyNum: int, at: int): int option = {
+    var r, omegaP, zd1, num, den, inv;
+
+    omegaP <@ Modexp.mid(OMEGA, polyNum);
+    zd1 <- (at^DOMAIN_SIZE - 1) %% R;
+    
+    if(zd1 = 0) {
+      r <- None;
+    } else {
+      num <- (omegaP * zd1) %% R;
+      den <- (DOMAIN_SIZE * (at - omegaP)) %% R;
+      inv <- den^(R - 2) %% R;
+      r <- Some ((num * inv) %% R);
+    }  
+    return r;
   }
 }.
 
@@ -69,8 +117,33 @@ lemma evaluateLagrangePolyOutOfDomain_extracted_equiv_low:
         call revertWithMessage_extracted_equiv_low. skip. by progress.
         sp. skip. by progress.
     qed.
-        
 
-        
-        
-        
+lemma evaluateLagrangePolyOutOfDomain_low_equiv_mid (memory : mem) (poly256 at256 r: uint256):
+equiv [
+    EvaluateLagrangePolyOutOfDomain.low ~ EvaluateLagrangePolyOutOfDomain.mid :
+      arg{1} = (poly256, at256) /\
+      arg{2} = (to_uint poly256, to_uint at256)%W256 /\
+      !Primops.reverted{1} /\
+      Primops.memory{1} = memory
+      ==>
+      (
+        !Primops.reverted{1} /\
+        Primops.memory{1} = (modexp_memory_footprint memory poly256 at256 res{1}) /\
+        res{2} = Some (to_uint res{1})%W256)
+      \/
+      (
+        Primops.reverted{1} /\
+        ((W256.to_uint at256)^DOMAIN_SIZE - 1) %% Constants.R = 0 /\
+        res{2} = None
+      )
+    ].
+proof. proc.
+seq 2 1 : (#pre /\ omegaPower{1} = W256.of_int omegaP{2}).
+seq 1 0 : (#pre /\ omegaPower{1} = W256.one). wp. skip. auto.
+case (bool_of_uint256 polyNum{1}).
+rcondt{1} 1. by progress.
+call (modexp_low_equiv_mid memory (W256.of_int OMEGA) poly256).
+skip. progress. smt. admit. (* HERE *)
+rcondf{1} 1. by progress.
+inline Modexp.mid. wp. skip. progress. rewrite /bool_of_uint256 in H0. by smt.
+
